@prefix time: <http://www.w3.org/2006/time#>.
@prefix dct: <http://purl.org/dc/terms/> .
@prefix cc: <http://creativecommons.org/ns#> .
@prefix xsd: <http://www.w3.org/2001/XMLSchema#> .
@prefix rdf: <http://www.w3.org/1999/02/22-rdf-syntax-ns#> .
@prefix rdfs: <http://www.w3.org/2000/01/rdf-schema#> .
@prefix skos: <http://www.w3.org/2004/02/skos/core#> .
@prefix era-organisation-roles: <http://data.europa.eu/949/concepts/organisation-roles/> .

## ORG roles concept scheme ## 

era-organisation-roles:OrgRoles a skos:ConceptScheme ;
	dct:issued "2024-07-31"^^xsd:date ;
    dct:modified "2024-09-04"^^xsd:date ;
   	cc:license <https://creativecommons.org/licenses/by/4.0/> ;
    rdfs:comment "Organisation roles used in different domains at ERA"@en ;
    rdfs:label "Organisation roles"@en ;
    skos:prefLabel "Organisation roles"@en ;
    dct:title "Concept scheme grouping roles held by organisations"@en ;
	skos:hasTopConcept era-organisation-roles:IM, era-organisation-roles:RU , era-organisation-roles:Owner,
	era-organisation-roles:Keeper, era-organisation-roles:Applicant, era-organisation-roles:ECM, era-organisation-roles:Manufacturer,
    era-organisation-roles:NSA ;	
		.


era-organisation-roles:IM a skos:Concept ;
        skos:inScheme era-organisation-roles:OrgRoles ;
		skos:prefLabel "Infrastructure Manager"@en;
		skos:altLabel "IM"@en ; 
        skos:notation "IM"^^xsd:string ;
		skos:topConceptOf era-organisation-roles:OrgRoles ; 
		skos:definition """ A body or firm responsible for the operation, maintenance and renewal of railway infrastructure on a network, as well as responsible for participating in its development as determined by the Member State within the framework of its general policy on development and financing of infrastructure"""@en ;
		dct:source <http://data.europa.eu/eli/dir/2012/34/2019-01-01> ; 
		.
		

era-organisation-roles:RU a skos:Concept ;
		skos:prefLabel "Railway Undertaking"@en ;
		skos:altLabel "RU"@en ;
        skos:notation "RU"^^xsd:string ;
		skos:inScheme era-organisation-roles:OrgRoles ;
		skos:topConceptOf era-organisation-roles:OrgRoles ;
		skos:definition """ 
		 Any public or private undertaking licensed according to this Directive, the principal business of which is to provide services for the transport of goods and/or passengers by rail with a requirement that the undertaking ensure traction; this also includes undertakings which provide traction only
		 """@en ;
		dct:source <http://data.europa.eu/eli/dir/2012/34/2019-01-01> ;
		.
		
era-organisation-roles:Owner a skos:Concept; 
		skos:prefLabel "Railway Vehicle Owner"@en ; 
		skos:inScheme era-organisation-roles:OrgRoles ;
		skos:altLabel "Owner"@en;
        skos:notation "Owner"^^xsd:string ;
		skos:topConceptOf era-organisation-roles:OrgRoles ;
		skos:definition "The natural or legal person being the owner of a vehicle exploited as a means of transport and is registered as such in a vehicle register referred to in Article 47";
        dct:references <http://data.europa.eu/eli/dir/2016/797/oj>, <http://data.europa.eu/eli/dir/2016/797/2020-05-28>;
  		.

era-organisation-roles:Keeper   a skos:Concept; 
			skos:inScheme era-organisation-roles:OrgRoles ;
			skos:prefLabel "Railway Vehicle Keeper"@en; 
			skos:topConceptOf era-organisation-roles:OrgRoles ;
			skos:definition "The natural or legal person that, being the owner of a vehicle or having the right to use it, exploits the vehicle as a means of transport and is registered as such in a vehicle register"@en ;
			dct:references <http://data.europa.eu/eli/dir/2016/797/oj>,  <http://data.europa.eu/eli/dir/2016/797/2020-05-28>;
            skos:notation "Keeper"^^xsd:string ;
			skos:altLabel "Keeper"@en;
			.

era-organisation-roles:Applicant a skos:Concept; 
			skos:inScheme era-organisation-roles:OrgRoles ;
			skos:topConceptOf era-organisation-roles:OrgRoles ;
			skos:prefLabel "Applicant"@en;
            skos:notation "Applicant"^^xsd:string ;
			skos:definition """ A natural or legal person requesting an authorisation, be it a railway undertaking, an infrastructure manager or any other person or legal entity, such as a manufacturer, an owner or a keeper """@en, 
			   """ a natural or legal person requesting the Agency's decision for the approval of the technical solutions envisaged for the ERTMS track-side equipment projects """@en ;
			
			dct:references <http://data.europa.eu/eli/dir/2016/797/oj>,  <http://data.europa.eu/eli/dir/2016/797/2020-05-28> ;
			.

era-organisation-roles:ECM a skos:Concept;
			  skos:inScheme era-organisation-roles:OrgRoles ; 
			  skos:prefLabel "Entity in charge of maintenance"@en ; 
			  skos:topConceptOf era-organisation-roles:OrgRoles ;
			  skos:definition """An entity in charge of the maintenance of a vehicle,  and registered as such in a vehicle register referred to in Article 47 of Directive (EU) 2016/797"""@en ;
              skos:scopeNote """ As defined in Article 3, point (20) of Directive (EU) 2016/798 and certified in accordance with Article 3 of Implementing Regulation (EU) 2019/779 """@en ; 
			  skos:narrower era-organisation-roles:ECM-b , era-organisation-roles:ECM-c, era-organisation-roles:ECM-d ; 
			  dct:references <http://data.europa.eu/eli/dir/2016/797/oj>, <http://data.europa.eu/eli/dir/2016/797/2020-05-28>;
              skos:notation "ECM"^^xsd:string ;
			  skos:altLabel "ECM"@en .

era-organisation-roles:ECM-b  a skos:Concept ;
		skos:prefLabel "ECM outsourcing the function provided for in Article 14(3), point (b) of Directive (EU) 2016/798 "@en ;
		skos:scopeNote """ ECM outsourcing the function provided for in Article 14(3), point (b) of Directive (EU) 2016/798 in accordance with Article 9 of Implementing Regulation (EU) 2019/779 """@en ;
        skos:notation "ECM-b"^^xsd:string ;
		skos:broader era-organisation-roles:ECM ;  
		skos:inScheme era-organisation-roles:OrgRoles ; 
        .
		
era-organisation-roles:ECM-c  a skos:Concept ;
		skos:prefLabel "ECM outsourcing the function defined in Article 14(3), point (c) of Directive (EU) 2016/798 "@en ;
		skos:scopeNote """ ECM outsourcing the function defined in Article 14(3), point (c) of Directive (EU) 2016/798 in accordance with Article 9 of Implementing Regulation (EU) 2019/779 """@en ;
        skos:notation "ECM-c"^^xsd:string ;
		skos:broader era-organisation-roles:ECM ;  
		skos:inScheme era-organisation-roles:OrgRoles ; 
        .
	
era-organisation-roles:ECM-d  a skos:Concept ;
		skos:prefLabel "ECM outsourcing the function defined in Article 14(3), point (d) of Directive (EU) 2016/798  "@en ;
		skos:scopeNote """ ECM outsourcing the function defined in Article 14(3), point (d) of Directive (EU) 2016/798 in accordance with Article 9 of Implementing Regulation (EU) 2019/779 """@en ;
        skos:notation "ECM-d"^^xsd:string ;
		skos:broader era-organisation-roles:ECM ;  
		skos:inScheme era-organisation-roles:OrgRoles ; 
        .


era-organisation-roles:MWS a skos:Concept;
			  skos:inScheme era-organisation-roles:OrgRoles ; 
			  skos:prefLabel "Maintenance workshop"@en ; 
			  skos:scopeNote """ MWS performing the functions defined in Article 14(3), points (b), (c) and (d) of Directive (EU) 2016/798 in accordance with Article 9 of Implementing Regulation (EU) 2019/779 """@en ; 
              skos:notation "MWS"^^xsd:string ;
			  skos:narrower era-organisation-roles:MWS-b , era-organisation-roles:MSW-c, era-organisation-roles:MSW-d ; 
			  skos:topConceptOf era-organisation-roles:OrgRoles;
			  skos:definition """An entity in charge of the maintenance of a vehicle,  and registered as such in a vehicle register referred to in Article 47 of Directive (EU) 2016/797"""@en ;
			  dct:references <http://data.europa.eu/eli/dir/2016/798/oj>, <http://data.europa.eu/eli/reg_impl/2019/779/oj>; 
			  skos:altLabel "MWS"@en .


era-organisation-roles:MWS-b a skos:Concept;
			  skos:inScheme era-organisation-roles:OrgRoles;
			  skos:prefLabel "MWS performing the function defined in Article 14(3), points (b) of Directive (EU) 2016/798"@en ; 
              skos:notation "MWS-b"^^xsd:string ;
			  skos:broader era-organisation-roles:MWS ;
			  skos:scopeNote """ MWS performing the function defined in Article 14(3), points (b) of Directive (EU) 2016/798, in accordance with Article 9 of Implementing Regulation (EU) 2019/779 """@en ;
			  .

era-organisation-roles:MWS-c a skos:Concept;
			  skos:inScheme era-organisation-roles:OrgRoles;
			  skos:prefLabel "MWS performing the function defined in Article 14(3), points (c) of Directive (EU) 2016/798"@en ; 
              skos:notation "MWS-c"^^xsd:string ;
			  skos:broader era-organisation-roles:MWS ;
			  skos:scopeNote """ MWS performing the function defined in Article 14(3), points (c) of Directive (EU) 2016/798, in accordance with Article 9 of Implementing Regulation (EU) 2019/779 """@en ;
			  .


era-organisation-roles:MWS-d a skos:Concept;
			  skos:inScheme era-organisation-roles:OrgRoles;
			  skos:prefLabel "MWS performing the function defined in Article 14(3), points (d) of Directive (EU) 2016/798"@en ; 
              skos:notation "MWS-d"^^xsd:string ;
			  skos:broader era-organisation-roles:MWS ;
			  skos:scopeNote """ MWS performing the function defined in Article 14(3), points (d) of Directive (EU) 2016/798, in accordance with Article 9 of Implementing Regulation (EU) 2019/779 """@en .

era-organisation-roles:Manufacturer   a skos:Concept ; 
			skos:inScheme era-organisation-roles:OrgRoles ;
            skos:notation "Manufacturer"^^xsd:string ;
			skos:prefLabel "Manufacturer"@en; 
			skos:topConceptOf era-organisation-roles:OrgRoles ;
			skos:definition """
				Any natural or legal person who manufactures a product in the form of interoperability constituents, subsystems or vehicles, or has it designed or manufactured, and markets it under his name or trademark
			"""@en ;
			
			dct:references <http://data.europa.eu/eli/dir/2016/797/2020-05-28> ; 
		    .

era-organisation-roles:NSA   a skos:Concept;
		skos:inScheme era-organisation-roles:OrgRoles ;
		skos:topConceptOf era-organisation-roles:OrgRoles ;
        skos:definition """ 
		 		(a) the national body entrusted with the tasks regarding railway safety in accordance with this Directive;
				(b) any body entrusted by several Member States with the tasks referred to in point (a) in order to ensure a unified safety regime;
				(c) any body entrusted by a Member State and a third country with the tasks referred to in point (a) in order to ensure a unified safety regime, provided that the Union has concluded an agreement to this effect with the third country concerned or that that Member State has concluded such 
			agreement in accordance with an empowerment granted by the Union to that effect;
		         """@en ;
		skos:prefLabel "National safety authority"@en ;
        skos:notation "NSA"^^xsd:string ;
		skos:altLabel "NSA"@en ;
        skos:scopeNote " National safety authority, as defined in Article 3, point (7) of Directive (EU) 2016/798"@en ;
		dct:source <http://data.europa.eu/eli/dir/2016/798/2020-10-23> ;
		.
		